Change the base case for the iff proof

Translation.thy
@@ -11,6 +11,62 @@ definition deducible :: "'c frege \<Rightarrow> ('c formula) set \<Rightarrow> '
   "deducible F asms c n \<longleftrightarrow>
      (\<exists> p. valid_proof F p \<and> assumptions p \<subseteq> asms \<and> thesis p = c \<and> len_proof p \<le> n)"
 
+lemma eval_sub_formula:
+  "eval al val (sub_formula sub f) = eval al (\<lambda>v. eval al val (sub v)) f"
+proof (induction f)
+  case (Atom a)
+  show ?case by simp
+next
+  case (Conn c zs)
+  have step: "\<And>x. x \<in> set zs \<Longrightarrow>
+       eval al val (sub_formula sub x) = eval al (\<lambda>v. eval al val (sub v)) x"
+    using Conn.IH by blast
+  have map_eq: "map (eval al val \<circ> sub_formula sub) zs =
+                map (eval al (\<lambda>v. eval al val (sub v))) zs"
+  proof (rule map_cong)
+    show "zs = zs" by (rule refl)
+  next
+    fix x assume x_in: "x \<in> set zs"
+    show "(eval al val \<circ> sub_formula sub) x = eval al (\<lambda>v. eval al val (sub v)) x"
+      using step[OF x_in] by (simp add: comp_def)
+  qed
+  have "eval al val (sub_formula sub (Conn c zs)) =
+        conn_evals al c (map (eval al val \<circ> sub_formula sub) zs)"
+    by (simp add: comp_def)
+  also have "\<dots> = conn_evals al c (map (eval al (\<lambda>v. eval al val (sub v))) zs)"
+    by (simp only: map_eq)
+  also have "\<dots> = eval al (\<lambda>v. eval al val (sub v)) (Conn c zs)"
+    by simp
+  finally show ?case .
+qed
+
+lemma fresh_distinct_atoms_exist:
+  "\<exists>vs :: string list.
+       length vs = n \<and> distinct vs \<and> ''a'' \<notin> set vs \<and> ''b'' \<notin> set vs"
+proof (induction n)
+  case 0
+  show ?case by (rule exI[where x="[]"]) simp
+next
+  case (Suc n)
+  obtain vs :: "string list" where
+    vs_props: "length vs = n" "distinct vs"
+              "''a'' \<notin> set vs" "''b'' \<notin> set vs"
+    using Suc.IH by blast
+  have inf_strings: "infinite (UNIV :: string set)"
+    by (simp add: infinite_UNIV_listI)
+  have finite_avoid: "finite (set vs \<union> {''a'', ''b''})"
+    using vs_props by simp
+  obtain x :: string where x_fresh: "x \<notin> set vs \<union> {''a'', ''b''}"
+    using inf_strings finite_avoid
+    by (meson ex_new_if_finite finite.emptyI finite.insertI finite_UnI finite_set)
+  let ?vs' = "x # vs"
+  have "length ?vs' = Suc n" using vs_props by simp
+  moreover have "distinct ?vs'" using vs_props x_fresh by auto
+  moreover have "''a'' \<notin> set ?vs'" using vs_props x_fresh by auto
+  moreover have "''b'' \<notin> set ?vs'" using vs_props x_fresh by auto
+  ultimately show ?case by blast
+qed
+
 locale frege_balancing =
   fixes F :: "'c frege"
   assumes "frege_system F"
@@ -49,18 +105,185 @@ fun distinguished :: "'c formula \<Rightarrow> string \<Rightarrow> bool" where
         (\<exists>! i. i < length fs \<and> contains_atom (fs ! i) h)
       \<and> (\<forall> f \<in> set fs. distinguished f h))"
 
+(*
+  We prove the existence of a fixed proof for congruence of each connective,
+  but to be able to say that this contributes only a constant factor we
+  designate a "canonical" instantiation of a connective and variables as children
+*)
+definition canonical_atoms :: "'c \<Rightarrow> string list" where
+  "canonical_atoms c = (SOME vs.
+       length vs = arity (alphabet F) c
+     \<and> distinct vs
+     \<and> ''a'' \<notin> set vs
+     \<and> ''b'' \<notin> set vs)"
+
+definition canonical_conn :: "'c \<Rightarrow> 'c formula" where
+  "canonical_conn c = Conn c (map Atom (canonical_atoms c))"
+
+lemma canonical_atoms_spec:
+  shows "length (canonical_atoms c) = arity (alphabet F) c \<and>
+         distinct (canonical_atoms c) \<and>
+         ''a'' \<notin> set (canonical_atoms c) \<and>
+         ''b'' \<notin> set (canonical_atoms c)"
+proof -
+  have ex: "\<exists>vs :: string list.
+              length vs = arity (alphabet F) c \<and> distinct vs
+            \<and> ''a'' \<notin> set vs \<and> ''b'' \<notin> set vs"
+    using fresh_distinct_atoms_exist by blast
+  show ?thesis
+    unfolding canonical_atoms_def using someI_ex[OF ex] .
+qed
+
 lemma iff_congruent_base:
-  fixes c  :: 'c
-    and fs :: "'c formula list"
-  shows "\<forall> \<phi> \<psi>. \<forall> i < length fs.
-          let sub  = \<lambda>v. if v = ''a'' then \<phi> else if v = ''b'' then \<psi> else Atom v;
-              sub' = \<lambda>v. if v = ''a'' then Conn c (fs[i := \<phi>])
-                         else if v = ''b'' then Conn c (fs[i := \<psi>])
-                         else Atom v
-          in \<exists> pr. valid_proof F pr \<and>
-                   assumptions pr = {sub_formula sub conn_iff} \<and>
-                   thesis pr = sub_formula sub' conn_iff"
-  sorry
+  fixes c :: 'c and i :: nat
+  assumes i_bound: "i < arity (alphabet F) c"
+  shows "\<exists>pr. valid_proof F pr \<and>
+              assumptions pr = {conn_iff} \<and>
+              thesis pr = sub_formula
+                (\<lambda>v. if v = ''a''
+                       then Conn c ((map Atom (canonical_atoms c))[i := Atom ''a''])
+                     else if v = ''b''
+                       then Conn c ((map Atom (canonical_atoms c))[i := Atom ''b''])
+                     else Atom v)
+                conn_iff"
+proof -
+  let ?atoms = "canonical_atoms c"
+  let ?children_a = "(map Atom ?atoms)[i := Atom ''a'']"
+  let ?children_b = "(map Atom ?atoms)[i := Atom ''b'']"
+  let ?sub' = "\<lambda>v. if v = ''a'' then Conn c ?children_a
+                  else if v = ''b'' then Conn c ?children_b
+                  else Atom v"
+  let ?al = "alphabet F"
+
+  have atoms_len: "length ?atoms = arity (alphabet F) c"
+    using canonical_atoms_spec by simp
+  hence i_lt_atoms: "i < length ?atoms" using i_bound by simp
+  have i_lt_map: "i < length (map Atom ?atoms)" using i_lt_atoms by simp
+
+  have fs_F: "frege_system F"
+    by (meson frege_balancing_axioms frege_balancing_def)
+
+  have conn_iff_equiv: "formulas_equiv conn_iff ?al iff_dm dm_alphabet"
+    unfolding conn_iff_def using someI_ex[OF conn_iff_spec] .
+
+  have iff_dm_eval: "\<And>v. eval dm_alphabet v iff_dm = (v ''a'' = v ''b'')"
+    unfolding iff_dm_def dm_alphabet_def by auto
+
+  have sem_valid: "\<forall>val. eval ?al val conn_iff \<longrightarrow>
+                         eval ?al val (sub_formula ?sub' conn_iff)"
+  proof (intro allI impI)
+    fix val :: "string \<Rightarrow> bool"
+    assume assm: "eval ?al val conn_iff"
+    let ?v2 = "\<lambda>v. eval ?al val (?sub' v)"
+
+    have eval1: "eval ?al val conn_iff = (val ''a'' = val ''b'')"
+    proof -
+      have "eval ?al val conn_iff = eval dm_alphabet val iff_dm"
+        using conn_iff_equiv unfolding formulas_equiv_def by simp
+      also have "\<dots> = (val ''a'' = val ''b'')" using iff_dm_eval .
+      finally show ?thesis .
+    qed
+
+    have ab_eq: "val ''a'' = val ''b''" using assm eval1 by simp
+
+    have sub_eval2: "eval ?al val (sub_formula ?sub' conn_iff) = (?v2 ''a'' = ?v2 ''b'')"
+    proof -
+      have "eval ?al val (sub_formula ?sub' conn_iff) = eval ?al ?v2 conn_iff"
+        by (rule eval_sub_formula)
+      also have "\<dots> = eval dm_alphabet ?v2 iff_dm"
+        using conn_iff_equiv unfolding formulas_equiv_def by simp
+      also have "\<dots> = (?v2 ''a'' = ?v2 ''b'')"
+        using iff_dm_eval .
+      finally show ?thesis .
+    qed
+
+    have v2a: "?v2 ''a'' = eval ?al val (Conn c ?children_a)" by simp
+    have v2b: "?v2 ''b'' = eval ?al val (Conn c ?children_b)" by simp
+
+    have map_eq: "map (eval ?al val) ?children_a = map (eval ?al val) ?children_b"
+    proof (rule nth_equalityI)
+      show "length (map (eval ?al val) ?children_a) =
+            length (map (eval ?al val) ?children_b)"
+        by simp
+    next
+      fix j
+      assume j_bound: "j < length (map (eval ?al val) ?children_a)"
+      hence j_lt_map: "j < length (map Atom ?atoms)" by simp
+      have nth_a: "map (eval ?al val) ?children_a ! j = eval ?al val (?children_a ! j)"
+        using j_lt_map by simp
+      have nth_b: "map (eval ?al val) ?children_b ! j = eval ?al val (?children_b ! j)"
+        using j_lt_map by simp
+      show "map (eval ?al val) ?children_a ! j = map (eval ?al val) ?children_b ! j"
+      proof (cases "j = i")
+        case True
+        have a_at_j: "?children_a ! j = Atom ''a''"
+          using True i_lt_map by simp
+        have b_at_j: "?children_b ! j = Atom ''b''"
+          using True i_lt_map by simp
+        have lhs: "map (eval ?al val) ?children_a ! j = val ''a''"
+        proof -
+          have "map (eval ?al val) ?children_a ! j = eval ?al val (?children_a ! j)"
+            using nth_a .
+          also have "\<dots> = eval ?al val (Atom ''a'')"
+            using a_at_j by (rule arg_cong)
+          also have "\<dots> = val ''a''" by simp
+          finally show ?thesis .
+        qed
+        have rhs: "map (eval ?al val) ?children_b ! j = val ''b''"
+        proof -
+          have "map (eval ?al val) ?children_b ! j = eval ?al val (?children_b ! j)"
+            using nth_b .
+          also have "\<dots> = eval ?al val (Atom ''b'')"
+            using b_at_j by (rule arg_cong)
+          also have "\<dots> = val ''b''" by simp
+          finally show ?thesis .
+        qed
+        show ?thesis using lhs rhs ab_eq by simp
+      next
+        case False
+        have a_at_j: "?children_a ! j = (map Atom ?atoms) ! j"
+          using False j_lt_map by (simp add: nth_list_update)
+        have b_at_j: "?children_b ! j = (map Atom ?atoms) ! j"
+          using False j_lt_map by (simp add: nth_list_update)
+        have lhs: "map (eval ?al val) ?children_a ! j = eval ?al val ((map Atom ?atoms) ! j)"
+        proof -
+          have "map (eval ?al val) ?children_a ! j = eval ?al val (?children_a ! j)"
+            using nth_a .
+          also have "\<dots> = eval ?al val ((map Atom ?atoms) ! j)"
+            using a_at_j by (rule arg_cong)
+          finally show ?thesis .
+        qed
+        have rhs: "map (eval ?al val) ?children_b ! j = eval ?al val ((map Atom ?atoms) ! j)"
+        proof -
+          have "map (eval ?al val) ?children_b ! j = eval ?al val (?children_b ! j)"
+            using nth_b .
+          also have "\<dots> = eval ?al val ((map Atom ?atoms) ! j)"
+            using b_at_j by (rule arg_cong)
+          finally show ?thesis .
+        qed
+        show ?thesis using lhs rhs by simp
+      qed
+    qed
+
+    have conn_eq:
+      "eval ?al val (Conn c ?children_a) = eval ?al val (Conn c ?children_b)"
+      using map_eq by simp
+
+    from conn_eq v2a v2b have v2_eq: "?v2 ''a'' = ?v2 ''b''" by simp
+    thus "eval ?al val (sub_formula ?sub' conn_iff)"
+      using sub_eval2 by simp
+  qed
+
+  have one_premise:
+    "\<forall>val. (\<forall>f \<in> {conn_iff}. eval ?al val f) \<longrightarrow>
+           eval ?al val (sub_formula ?sub' conn_iff)"
+    using sem_valid by simp
+
+  show "\<exists>pr. valid_proof F pr \<and>
+             assumptions pr = {conn_iff} \<and>
+             thesis pr = sub_formula ?sub' conn_iff"
+    using one_premise frege_system.impl_complete[OF fs_F] by blast
+qed
 
 (* lemma 3.2: *)
 lemma iff_congruent:
